src/ManCompSoundness_newManGen.v
@@ -1,0 +1,1516 @@
+Require Import Manifest Manifest_Compiler Manifest_Generator 
+  Maps Term_Defs List Cvm_St Cvm_Impl ErrorStMonad_Coq StructTactics Cvm_Monad EqClass Manifest_Admits.
+Require Import Manifest_Generator_Facts Executable_Defs_Prop Executable_Facts_Dist.
+
+Require Import Auto.
+Import ListNotations.
+
+
+(* map_get (minify_mapD Local_Plcs (fun _ : Plc => false)) p1 *)
+
+Fixpoint knowsOf_asps (tp : Plc) (p : Plc) (t : Term) : list ASP_ID :=
+  match t with
+  | asp a =>
+    if (eqb tp p)
+    then 
+      (match a with
+      | ASPC _ _ par =>
+          match par with
+          | asp_paramsC i _ targp targid => [i]
+          end
+      | SIG => [sig_aspid]
+      | HSH => [hsh_aspid]
+      | ENC p => [enc_aspid]
+      | _ => nil
+      end)
+    else nil
+  | att p' t' => knowsOf_asps tp p' t'
+  | lseq t1 t2 =>
+      knowsOf_asps tp p t1 ++ knowsOf_asps tp p t2
+  | bseq _ t1 t2 =>
+      knowsOf_asps tp p t1 ++ knowsOf_asps tp p t2
+  | bpar _ t1 t2 =>
+      knowsOf_asps tp p t1 ++ knowsOf_asps tp p t2
+  end.
+
+Fixpoint knowsOf_uuid' (tp : Plc) (p:Plc) (t:Term)  : list Plc :=
+  match t with
+  | asp a => nil
+  | att p' t' => 
+      if (eqb tp p)
+      then (* We are the top-level place, we need to know this *) 
+        p' :: knowsOf_uuid' tp p' t'
+      else knowsOf_uuid' tp p' t'
+  | lseq t1 t2 =>
+     knowsOf_uuid' tp p t1 ++ knowsOf_uuid' tp p t2
+  | bseq _ t1 t2 =>
+     knowsOf_uuid' tp p t1 ++ knowsOf_uuid' tp p t2
+  | bpar _ t1 t2 =>
+     knowsOf_uuid' tp p t1 ++ knowsOf_uuid' tp p t2
+  end.
+
+Fixpoint knowsOf_uuid'' (tp : Plc) (p:Plc) (t:Term)  : list Plc :=
+  match t with
+  | asp a => nil
+  | att p' t' => 
+      if (eqb tp p)
+      then (* We are the top-level place, we need to know this *) 
+        p' :: knowsOf_uuid'' p' p t'
+      else knowsOf_uuid'' p' p t'
+  | lseq t1 t2 =>
+     knowsOf_uuid'' tp p t1 ++ knowsOf_uuid'' tp p t2
+  | bseq _ t1 t2 =>
+     knowsOf_uuid'' tp p t1 ++ knowsOf_uuid'' tp p t2
+  | bpar _ t1 t2 =>
+     knowsOf_uuid'' tp p t1 ++ knowsOf_uuid'' tp p t2
+  end.
+
+Fixpoint mentioned_places (t : Term) : list Plc :=
+  match t with
+  | asp a => nil
+  | att p' t' => 
+      p' :: mentioned_places t'
+  | lseq t1 t2 =>
+      mentioned_places t1 ++ mentioned_places t2
+  | bseq _ t1 t2 =>
+      mentioned_places t1 ++ mentioned_places t2
+  | bpar _ t1 t2 =>
+      mentioned_places t1 ++ mentioned_places t2
+  end.
+
+Fixpoint knowsOf_pubkey' (tp : Plc) (p : Plc) (t : Term) : list ASP_ID :=
+  match t with
+  | asp a =>
+    match a with
+    | ENC p => if (eqb tp p) then [p] else nil
+    | _ => nil
+    end
+  | att p' t' => knowsOf_pubkey' tp p' t'
+  | lseq t1 t2 =>
+      knowsOf_pubkey' tp p t1 ++ knowsOf_pubkey' tp p t2
+  | bseq _ t1 t2 =>
+      knowsOf_pubkey' tp p t1 ++ knowsOf_pubkey' tp p t2
+  | bpar _ t1 t2 =>
+      knowsOf_pubkey' tp p t1 ++ knowsOf_pubkey' tp p t2
+  end.
+
+Fixpoint static_executable_manifest (t : Term) (m : Manifest) : Prop :=
+  match t with
+  | asp a => 
+      match a with
+      | ASPC _ _ par =>
+          match par with
+          | asp_paramsC i _ targp targid => 
+              In i (asps m)
+          end
+      | SIG => In sig_aspid (asps m)
+      | HSH => In hsh_aspid (asps m)
+      | ENC p => In enc_aspid (asps m) /\ In p (pubKeyPlcs m)
+      | NULL => True
+      | CPY => True 
+      end
+  | att p' t => In p' (uuidPlcs m)
+  | lseq t1 t2 => static_executable_manifest t1 m /\ static_executable_manifest t2 m
+  | bseq _ t1 t2 => static_executable_manifest t1 m /\ static_executable_manifest t2 m
+  | bpar _ t1 t2 => static_executable_manifest t1 m /\ static_executable_manifest t2 m
+  end.
+
+Ltac grind :=
+  repeat (try break_match; simpl in *; intuition; subst; eauto; try congruence);
+  repeat find_injection; subst;
+  simpl in *; intuition; eauto.
+
+Ltac breq l r :=
+  let E := fresh "Heq" in
+  destruct (eqb l r) eqn:E;
+  try rewrite E in *;
+  try (rewrite eqb_leibniz in *; subst; simpl in *; intuition; eauto; try congruence);
+  try (rewrite eqb_refl in *; subst; simpl in *; intuition; eauto; try congruence);
+  try (assert (l <> r) by (intros HC; rewrite <- eqb_leibniz in *; congruence)).
+
+Ltac unf :=
+  repeat (unfold asp_manifest_generator,
+    at_manifest_generator, knowsof_manifest_update,
+    asp_manifest_update, manifest_update_env,
+    aspid_manifest_update, update_manifest_policy_targ,
+    empty_Manifest in *
+  ); simpl in *; try (intuition; eauto; congruence).
+(* 
+
+Theorem man_gen_only_available_if_known : forall t p backEnv envM p',
+  map_get backEnv p' = None ->
+  manifest_generator' p t backEnv = envM ->
+  ((exists man, map_get envM p' = Some man) <-> In p' (knowsOf_uuid' p p' t)).
+Proof.
+  induction t; simpl in *; intuition; eauto; subst.
+  - unfold asp_manifest_generator, manifest_update_env, 
+      asp_manifest_update, aspid_manifest_update, update_manifest_policy_targ,
+      pubkey_manifest_update in *; simpl in *; destruct H1.
+    destruct a; simpl in *;
+    break_match; subst;
+    breq p p';
+    erewrite mapC_get_distinct_keys_from_set in H; intuition; eauto; try congruence.
+  - unfold asp_manifest_generator, manifest_update_env, 
+      asp_manifest_update, aspid_manifest_update, update_manifest_policy_targ,
+      pubkey_manifest_update in *; simpl in *.
+    destruct a; simpl in *;
+    repeat break_match; subst; simpl in *; eauto; try congruence;
+    try rewrite mapC_get_works; eexists; eauto.
+  - breq p0 p'.
+    unfold at_manifest_generator, manifest_update_env, knowsof_manifest_update in *;
+    simpl in *.
+    destruct (manifest_generator' p t
+            (map_set backEnv p0
+               (let
+                '{|
+                   my_abstract_plc := oldPlc;
+                   asps := oldasps;
+                   uuidPlcs := oldKnowsOf;
+                   pubKeyPlcs := oldContext;
+                   targetPlcs := oldTargets;
+                   policy := oldPolicy
+                 |} := match map_get backEnv p0 with
+                       | Some mm => mm
+                       | None => empty_Manifest
+                       end in
+                 {|
+                   my_abstract_plc := oldPlc;
+                   asps := oldasps;
+                   uuidPlcs := p :: oldKnowsOf;
+                   pubKeyPlcs := oldContext;
+                   targetPlcs := oldTargets;
+                   policy := oldPolicy
+                 |}))) eqn:E;
+    try (exfalso; eapply manifest_generator_never_empty; eauto; fail).
+    repeat break_match; simpl in *; eauto;
+    repeat break_match; simpl in *.
+    * destruct H1; repeat find_injection; simpl in *.
+      rewrite eqb_leibniz in *; subst.
+      assert (map_get (map_set backEnv p0
+         {|
+           my_abstract_plc := my_abstract_plc;
+           asps := asps;
+           uuidPlcs := p :: uuidPlcs;
+           pubKeyPlcs := pubKeyPlcs;
+           targetPlcs := targetPlcs;
+           policy := policy
+         |}) p' = None). admit.
+      pose proof (IHt _ _ _ _ H1 E).
+      assert (exists man, map_get ((p',x) :: e) p' = Some man). admit.
+      rewrite H2 in H3; intuition; eauto; subst.
+
+Theorem man_gen_only_available_if_known : forall t p backEnv envM p',
+  map_get backEnv p' = None ->
+  manifest_generator' p t backEnv = envM ->
+  ((exists man, map_get envM p' = Some man) <-> (In p' (knowsOf_uuid' p p' t) \/ p = p')).
+Proof.
+  induction t; simpl in *; intuition; eauto; subst.
+  - unfold asp_manifest_generator, manifest_update_env, 
+      asp_manifest_update, aspid_manifest_update, update_manifest_policy_targ,
+      pubkey_manifest_update in *; simpl in *. destruct H1.
+    destruct a; simpl in *;
+    break_match; subst;
+    breq p p';
+    erewrite mapC_get_distinct_keys_from_set in H; intuition; eauto; try congruence.
+  - unfold asp_manifest_generator, manifest_update_env, 
+      asp_manifest_update, aspid_manifest_update, update_manifest_policy_targ,
+      pubkey_manifest_update in *; simpl in *.
+    destruct a; simpl in *;
+    repeat break_match; subst; simpl in *; eauto; try congruence;
+    try rewrite mapC_get_works; eexists; eauto.
+  - breq p0 p'.
+    unfold at_manifest_generator, manifest_update_env, knowsof_manifest_update in *;
+    simpl in *.
+    destruct (manifest_generator' p t
+            (map_set backEnv p0
+               (let
+                '{|
+                   my_abstract_plc := oldPlc;
+                   asps := oldasps;
+                   uuidPlcs := oldKnowsOf;
+                   pubKeyPlcs := oldContext;
+                   targetPlcs := oldTargets;
+                   policy := oldPolicy
+                 |} := match map_get backEnv p0 with
+                       | Some mm => mm
+                       | None => empty_Manifest
+                       end in
+                 {|
+                   my_abstract_plc := oldPlc;
+                   asps := oldasps;
+                   uuidPlcs := p :: oldKnowsOf;
+                   pubKeyPlcs := oldContext;
+                   targetPlcs := oldTargets;
+                   policy := oldPolicy
+                 |}))) eqn:E;
+    try (exfalso; eapply manifest_generator_never_empty; eauto; fail).
+    repeat break_match; simpl in *; eauto;
+    repeat break_match; simpl in *.
+    * destruct H1; repeat find_injection; simpl in *.
+      rewrite eqb_leibniz in *; subst.
+      assert (map_get (map_set backEnv p0
+         {|
+           my_abstract_plc := my_abstract_plc;
+           asps := asps;
+           uuidPlcs := p :: uuidPlcs;
+           pubKeyPlcs := pubKeyPlcs;
+           targetPlcs := targetPlcs;
+           policy := policy
+         |}) p' = None). admit.
+      pose proof (IHt _ _ _ _ H1 E).
+      assert (exists man, map_get ((p',x) :: e) p' = Some man). admit.
+      rewrite H2 in H3; intuition; eauto; subst. *)
+
+    
+
+(* Theorem manifest_generator_impl_static_executable_manifest : forall t p backEnv envM,
+  (forall p' man,
+    map_get backEnv p' = Some man ->
+    static_executable_manifest t man) ->
+  manifest_generator' p t backEnv = envM ->
+  (forall p' man,
+    map_get envM p' = Some man ->
+    static_executable_manifest t man
+  ).
+Proof.
+  induction t; simpl in *; intuition; eauto.
+  - destruct a; simpl in *; intuition; eauto.
+    * destruct a; simpl in *; eauto.
+      unfold asp_manifest_generator, manifest_update_env, 
+        asp_manifest_update, aspid_manifest_update, 
+        update_manifest_policy_targ in *; simpl in *;
+      repeat break_match; simpl in *;
+      repeat find_injection.
+      ** eapply H in Heqo; simpl in *.
+  
+Qed. *)
+
+
+(* Theorem manifest_generator_works : forall t p backEnv envM,
+  manifest_generator' p t backEnv = envM ->
+  forall p' absMan,
+    map_get envM p' = Some absMan ->
+    ((forall (a : ASP_ID), In a (knowsOf_asps p p' t) -> In a (asps absMan)) /\ 
+     (forall (u : Plc), In u (knowsOf_uuid' p p' t) -> In u (uuidPlcs absMan)) /\
+     (forall (u : Plc), In u (knowsOf_pubkey' p p' t) -> In u (pubKeyPlcs absMan))).
+Proof.
+  intros t p stEnv.
+  pose proof (manifest_generator_executability_static' t p stEnv).
+  generalizeEverythingElse t.
+  induction t; simpl in *; intros.
+  - destruct a; simpl in *;
+    repeat break_match; simpl in *; intuition; eauto;
+    subst.
+    unfold canRunAsp_Env in *.
+
+
+  simpl in *.
+
+  induction t; simpl in *; intros.
+  - repeat break_match; simpl in *; intuition; subst; eauto; 
+    try congruence; unfold canRunAsp_Env in *; simpl in *; eauto;
+    try break_if; try (rewrite eqb_leibniz in *; subst; eauto); admit.
+  - eapply IHt in H as IH; simpl in *; intuition; eauto;
+    break_if; eauto; clear IHt; rewrite <- H in H0. clear H.
+    rewrite eqb_leibniz in *.
+    rewrite Heqb in *; clear Heqb; eauto; simpl in *;
+    intuition; rewrite H in *. clear H.
+    unfold at_manifest_generator, manifest_update_env, knowsof_manifest_update 
+      in *; repeat break_match; subst; simpl in *; intuition; eauto;
+    pose proof (man_gen_map_getter t u p'
+             {|
+               my_abstract_plc := my_abstract_plc;
+               asps := asps;
+               uuidPlcs := u :: uuidPlcs;
+               pubKeyPlcs := pubKeyPlcs;
+               targetPlcs := targetPlcs;
+               policy := policy
+             |} backEnv); destruct H; intuition; simpl in *; 
+    find_rewrite; find_injection; eauto.
+  - 
+    destruct (manifest_generator' p t1 backEnv) eqn:E1;
+    try (exfalso; eapply manifest_generator_never_empty; eauto; fail);
+    destruct (map_get (manifest_generator' p t1 backEnv) p') eqn:E2.
+    * rewrite E1 in E2;
+      pose proof (IHt1 p backEnv (p0 :: e) E1 _ _ E2).
+      pose proof (IHt2 p (p0 :: e) envM H _ _ H0);
+      intuition; rewrite in_app_iff in *; intuition; eauto;
+      clear IHt1 IHt2; admit.
+    * 
+    pose proof (man_gen_map_getter).
+    intuition; rewrite in_app_iff in *; intuition.
+    * destruct (manifest_generator' p t1 backEnv) eqn:E1;
+      try (exfalso; eapply manifest_generator_never_empty; eauto; fail);
+      destruct p0; simpl in *.
+      pose proof (IHt1 _ _ _ E1 p'); simpl in *;
+      break_if; try (rewrite eqb_leibniz in *; subst; intuition; eauto).
+      admit.
+      pose proof (man_gen_doesnt_kill_info).
+    pose proof (IHt1 _ _ _ E1). clear IHt1 E1.
+    destruct p0.
+    destruct (manifest_generator' p t2 ((p0, m) :: e)) eqn:E2;
+    try (exfalso; eapply manifest_generator_never_empty; eauto; fail).
+    pose proof (IHt2 _ _ _ E2); destruct p1; simpl in *. clear IHt2; simpl in *; subst.
+    simpl in *.
+    break_if; try (rewrite eqb_leibniz in *; subst; eauto; find_injection).
+    * intuition; eauto; rewrite in_app_iff in *; intuition; eauto.
+    simpl in *; intuition; eauto.
+    * eapply IHt1 in E1 as E'.
+    eapply IHt1 in E1.
+    destruct H; eapply IHt1 in H; eapply IHt2 in H1; eauto;
+    intuition; rewrite in_app_iff in *; intuition; eauto.
+  - destruct H; eapply IHt1 in H; eapply IHt2 in H1; eauto;
+    intuition; rewrite in_app_iff in *; intuition; eauto.
+  - destruct H; eapply IHt1 in H; eapply IHt2 in H1; eauto;
+    intuition; rewrite in_app_iff in *; intuition; eauto.
+Qed. *)
+
+
+Ltac cunf :=
+  repeat (unfold asp_manifest_generator,
+    asp_manifest_update,
+    aspid_manifest_update,
+    at_manifest_generator,
+    manifest_update_env,
+    knowsof_manifest_update,
+    update_manifest_policy_targ,
+    pubkey_manifest_update,
+    map_set;
+  simpl in *; eauto);
+  repeat break_match;
+  repeat find_injection;
+  subst;
+  repeat find_inversion;
+  try congruence;
+  simpl in *;
+  eauto.
+(* 
+Lemma man_gen_map_getter : forall t u preEnv p st postEnv,
+  map_get preEnv p = None ->
+  exists st', 
+    (map_get (manifest_generator' u t (preEnv ++ (p, st) :: postEnv)) p = Some st') /\
+    (forall x, In x st.(uuidPlcs) -> In x st'.(uuidPlcs)) /\
+    (forall x, In x st.(asps) -> In x st'.(asps)) /\
+    (forall x, In x st.(pubKeyPlcs) -> In x st'.(pubKeyPlcs)).
+Proof.
+
+  induction t; simpl in *; intuition; eauto.
+  - break_if.
+    * rewrite eqb_leibniz in *; subst;
+      break_match; try (edestruct @map_sandwich_not_none; eauto; fail);
+      eapply map_app_unfolder in Heqo; subst; eauto;
+      eexists; intuition; cunf.
+    * destruct (map_has_buried preEnv p st postEnv);
+      pose proof (map_app_unfolder preEnv p st postEnv _ H0 H); subst;
+      eexists; intuition; cunf.
+  - cunf.
+    * pose proof (IHt p ((u,
+         {|
+           my_abstract_plc := my_abstract_plc;
+           asps := asps;
+           uuidPlcs := p :: uuidPlcs;
+           pubKeyPlcs := pubKeyPlcs;
+           targetPlcs := targetPlcs;
+           policy := policy
+         |}) :: preEnv) p0 ).
+    cunf; eexists; intuition; eauto.
+      break_match.
+      admit.
+      
+      exfalso. eapply map_sandwich_not_none; eauto.
+      admit.
+      break_match; eexists; intuition; cunf; destruct a; 
+      pose proof (map_app_unfolder preEnv u st postEnv _ Heqo H); subst. *)
+
+(* Definition knowsOf_pubkey (p : Plc) (t : Term) : list ASP_ID :=
+  p :: (knowsOf_pubkey' p t). *)
+(* Lemma man_gen_doesnt_kill_info : forall t u p st absMan preEnv postEnv,
+  map_get 
+    (manifest_generator' u t
+      (preEnv ++ (p, st) :: postEnv)) p = Some absMan ->
+  map_get preEnv p = None ->
+  forall x,
+  In x (st.(uuidPlcs)) ->
+  In x (absMan.(uuidPlcs)).
+Proof.
+  induction t; simpl in *; intuition; eauto.
+  - break_if; unfold asp_manifest_update, aspid_manifest_update,
+      update_manifest_policy_targ, pubkey_manifest_update in *; simpl in *;
+    repeat break_match; repeat find_injection; simpl in *; eauto; try congruence;
+    try (rewrite eqb_leibniz in *; subst; simpl in *; eauto);
+    try (eapply map_app_unfolder in Heqo; subst; eauto; fail);
+    try (eapply map_sandwich_not_none in Heqo; exfalso; eauto; fail).
+    * eapply map_app_unfolder in H; subst; simpl in *; eauto.
+  - unfold at_manifest_generator, manifest_update_env, knowsof_manifest_update, map_set in *.
+    break_match.
+    destruct (eqb u p0) eqn:E.
+    * rewrite eqb_leibniz in *; subst.
+      pose proof (IHt p p0 {|
+             my_abstract_plc := my_abstract_plc;
+             asps := asps;
+             uuidPlcs := p :: uuidPlcs;
+             pubKeyPlcs := pubKeyPlcs;
+             targetPlcs := targetPlcs;
+             policy := policy
+           |} absMan nil (preEnv ++ (p0, st) :: postEnv)); simpl in *.
+      break_match; subst; simpl in *; intuition; eauto.
+      ** eapply map_app_unfolder in Heqo; eauto; destruct st; find_injection; eauto.
+      ** eapply map_sandwich_not_none in Heqo; exfalso; eauto.
+    * pose proof (IHt p p0 st absMan ((u,
+           {|
+             my_abstract_plc := my_abstract_plc;
+             asps := asps;
+             uuidPlcs := p :: uuidPlcs;
+             pubKeyPlcs := pubKeyPlcs;
+             targetPlcs := targetPlcs;
+             policy := policy
+           |}) :: preEnv) postEnv). rewrite app_comm_cons in *;
+           intuition; eapply H3; eauto.
+      simpl in *. rewrite eqb_symm. rewrite E; eauto.
+  - destruct (manifest_generator' u t1 (preEnv ++ (p, st) :: postEnv)) eqn:E;
+    try (exfalso; eapply manifest_generator_never_empty; eauto; fail);
+    destruct p0.
+    destruct (map_get ((p0, m) :: e) p) eqn:E1.
+    destruct (manifest_generator' u t2 (p0 :: e))
+
+    eapply (IHt1 u p st absMan preEnv postEnv); eauto.
+    destruct (manifest_generator' u t1 (preEnv ++ (p, st) :: postEnv)) eqn:E;
+    
+
+
+    (* * pose proof (IHt p p0 {|
+             my_abstract_plc := my_abstract_plc;
+             asps := asps;
+             uuidPlcs := p :: uuidPlcs;
+             pubKeyPlcs := pubKeyPlcs;
+             targetPlcs := targetPlcs;
+             policy := policy
+           |} absMan nil (preEnv ++ (p0, st) :: postEnv)); simpl in *;
+      eapply H2; eauto.
+      break_match; subst; simpl in *; intuition; eauto.
+      ** eapply map_app_unfolder in Heqo; eauto; destruct st; find_injection; eauto.
+      ** eapply map_sandwich_not_none in Heqo; exfalso; eauto.
+      intuition; eapply H2; intuition; eauto.
+     rewrite app_comm_cons in *; eapply IHt in H; eauto.
+    simpl in *.
+    pose proof (IHt p p0 st absMan ((u,
+           {|
+             my_abstract_plc := my_abstract_plc;
+             asps := asps;
+             uuidPlcs := p :: uuidPlcs;
+             pubKeyPlcs := pubKeyPlcs;
+             targetPlcs := targetPlcs;
+             policy := policy
+           |}) :: preEnv ) ).
+    rewrite <- H.
+    pose proof (IHt p u {|
+             my_abstract_plc := my_abstract_plc;
+             asps := asps;
+             uuidPlcs := p :: uuidPlcs;
+             pubKeyPlcs := pubKeyPlcs;
+             targetPlcs := targetPlcs;
+             policy := policy
+           |} absMan ((p0, st) :: backEnv)); intuition.
+    eapply IHt in H.
+    repeat find_injection; try find_contradiction. *)
+Admitted. *)
+
+(* Global Hint Resolve man_gen_doesnt_kill_info : core. *)
+
+(* Theorem executable_impl_precond : forall t p backEnv envM,
+  manifest_generator' p t backEnv = envM ->
+  (forall p' absMan,
+    map_get envM p' = Some absMan ->
+    ((forall (a : ASP_ID), In a (knowsOf_asps p p' t) -> In a (asps absMan)) /\ 
+     (forall (u : Plc), In u (knowsOf_uuid' p p' t) -> In u (uuidPlcs absMan)) /\
+     (forall (u : Plc), In u (knowsOf_pubkey' p p' t) -> In u (pubKeyPlcs absMan)))
+  ).
+Proof.
+  induction t; simpl in *; intros.
+  - repeat break_match; simpl in *; intuition; subst; eauto; 
+    try congruence; unfold canRunAsp_Env in *; simpl in *;
+    break_if; try (rewrite eqb_leibniz in *; subst; eauto);
+    admit.
+  - eapply IHt in H as IH; simpl in *; intuition; eauto;
+    break_if; eauto; clear IHt; rewrite <- H in H0. clear H.
+    rewrite eqb_leibniz in *.
+    rewrite Heqb in *; clear Heqb; eauto; simpl in *;
+    intuition; rewrite H in *. clear H.
+    unfold at_manifest_generator, manifest_update_env, knowsof_manifest_update,
+      map_set in *; repeat break_match; subst; simpl in *; intuition; eauto;
+    eapply man_gen_doesnt_kill_info with (preEnv := nil); eauto; simpl in *; eauto.
+  - intuition; rewrite in_app_iff in *; intuition.
+    * destruct (manifest_generator' p t1 backEnv) eqn:E1;
+      try (exfalso; eapply manifest_generator_never_empty; eauto; fail);
+      destruct p0; simpl in *.
+      pose proof (IHt1 _ _ _ E1 p'); simpl in *;
+      break_if; try (rewrite eqb_leibniz in *; subst; intuition; eauto).
+      pose proof (man_gen_doesnt_kill_info).
+    pose proof (IHt1 _ _ _ E1). clear IHt1 E1.
+    destruct p0.
+    destruct (manifest_generator' p t2 ((p0, m) :: e)) eqn:E2;
+    try (exfalso; eapply manifest_generator_never_empty; eauto; fail).
+    pose proof (IHt2 _ _ _ E2); destruct p1; simpl in *. clear IHt2; simpl in *; subst.
+    simpl in *.
+    break_if; try (rewrite eqb_leibniz in *; subst; eauto; find_injection).
+    * intuition; eauto; rewrite in_app_iff in *; intuition; eauto.
+    simpl in *; intuition; eauto.
+    * eapply IHt1 in E1 as E'.
+    eapply IHt1 in E1.
+    destruct H; eapply IHt1 in H; eapply IHt2 in H1; eauto;
+    intuition; rewrite in_app_iff in *; intuition; eauto.
+  - destruct H; eapply IHt1 in H; eapply IHt2 in H1; eauto;
+    intuition; rewrite in_app_iff in *; intuition; eauto.
+  - destruct H; eapply IHt1 in H; eapply IHt2 in H1; eauto;
+    intuition; rewrite in_app_iff in *; intuition; eauto.
+Admitted. *)
+
+Definition lib_supports_manifest (al : AM_Library) (am : Manifest) : Prop :=
+  (forall (a : ASP_ID), In a am.(asps) -> exists cb, Maps.map_get al.(Local_ASPS) a = Some cb) /\
+  (forall (up : Plc), In up am.(uuidPlcs) -> exists b, Maps.map_get al.(Local_Plcs) up = Some b) /\
+  (forall (pkp : Plc), In pkp am.(pubKeyPlcs) -> exists b, Maps.map_get al.(Local_PubKeys) pkp = Some b).
+
+Ltac unfolds :=
+  (* repeat monad_unfold; *)
+  repeat unfold manifest_generator, manifest_compiler, generate_ASP_dispatcher, 
+    generate_Plc_dispatcher, generate_PubKey_dispatcher,
+    generate_UUID_dispatcher, lib_supports_manifest, aspid_manifest_update,
+    sig_params, hsh_params, enc_params in *;
+  simpl in *; 
+  repeat (match goal with
+      | x : cvm_st |- _ => destruct x
+      | x : AM_Config |- _ => destruct x
+      | x : AM_Library |- _ => destruct x
+      | x : CallBackErrors |- _ => destruct x
+  end; simpl in *; eauto);
+  intuition.
+
+Theorem man_gen_aspid_in : forall a m,
+  In a (asps (aspid_manifest_update a m)).
+Proof.
+  induction m; simpl in *; eauto.
+Qed.
+
+
+
+(* Lemma stupid_map_killer : forall a Local_ASPS st_pl st_ev p t m l d,
+  (exists cb : CakeML_ASPCallback CallBackErrors, map_get Local_ASPS a = Some cb) ->
+  (match
+      map_get
+        (minify_mapC Local_ASPS
+            (fun x : ASP_ID =>
+            if
+              in_dec (EqClass_impl_DecEq ASP_ID) x (asps (aspid_manifest_update a (update_manifest_policy_targ p t m)))
+            then true
+            else false)) a
+        with
+        | Some cb =>
+            match cb (asp_paramsC a l p t) st_pl (encodeEvRaw (get_bits st_ev)) (get_bits st_ev) with
+            | errC c => match c with
+                        | messageLift _ => errC Runtime
+                        end
+            | resultC r => resultC r
+            end
+        | None => errC Unavailable
+        end = errC d) ->
+  d = Runtime.
+Proof.
+  destruct d; eauto; intros; repeat break_match; 
+  try congruence; clear H0.
+  destruct H; pose proof man_gen_aspid_in; eauto.
+  pose proof (H0 a). clear H0.
+  assert (Some x = None). {
+    rewrite <- H, <- Heqo.
+    clear Heqo H st_pl st_ev x l.
+    induction Local_ASPS; simpl in *; eauto.
+    rewrite IHLocal_ASPS. clear IHLocal_ASPS.
+    simpl in *.
+    destruct a0, (eqb a a0) eqn:E; simpl in *; eauto;
+    try (rewrite eqb_leibniz in E; subst; eauto).
+    - destruct (in_dec (EqClass_impl_DecEq ASP_ID) a0 (asps (aspid_manifest_update a0 (update_manifest_policy_targ p t m)))); simpl in *; try rewrite eqb_refl in *; eauto; try (pose proof (H1 (update_manifest_policy_targ p t m))); try congruence.
+    - destruct (in_dec (EqClass_impl_DecEq ASP_ID) a0 (asps (aspid_manifest_update a (update_manifest_policy_targ p t m)))); simpl in *; eauto; rewrite E; eauto.
+  }
+  congruence.
+Qed.
+
+
+Global Hint Resolve stupid_map_killer : core. *)
+Global Hint Resolve man_gen_aspid_in : core.
+
+(* 
+Lemma generated_uuid_plcs_not_none : forall (l : MapD Plc UUID) (p : Plc) t p0 backEnv p' absMan,
+  (map_get (manifest_generator' p t (at_manifest_generator p0 p backEnv)) p' = Some absMan) ->
+  (forall up : Plc, In up (uuidPlcs absMan) -> exists b : UUID, map_get l up = Some b) ->
+  (map_get (minify_mapD l 
+    (fun x : Plc => if in_dec (EqClass_impl_DecEq Plc) x (uuidPlcs absMan) then true else false)) p = None) ->
+  False.
+Proof.
+  induction l; simpl in *; intuition; eauto.
+  - admit.
+  - repeat (break_if; simpl in *; eauto; try congruence).
+    * admit.
+    * 
+    * pose proof (IHl _ _ _ _ _ _ H).
+      eapply IHl; eauto; intros.
+      destruct (H0 _ H2); break_if; eauto; invc H3.
+      rewrite eqb_leibniz in *; subst. *)
+
+Theorem filter_resolver : forall {A B} `{EqClass A} (m : MapC A B) a (filt : A -> bool),
+  (exists x, map_get m a = Some x) ->
+  filt a = true ->
+  exists x, map_get (minify_mapC m filt) a = Some x.
+Proof.
+  induction m; intuition; simpl in *;
+  destruct (eqb a a0) eqn:E.
+  - rewrite eqb_leibniz in E; subst. rewrite H1; simpl in *; rewrite eqb_refl; eauto.
+  - repeat break_match; simpl in *; 
+    try (pose proof eqb_symm; congruence);
+    simpl in *; eauto.
+    rewrite eqb_symm; rewrite E; eauto.
+Qed.
+
+
+Theorem filter_resolver_mapd : forall {A B} `{EqClass A, EqClass B} (m : MapC A B) a (filt : A -> bool),
+  (exists x, map_get m a = Some x) ->
+  filt a = true ->
+  exists x, map_get (minify_mapD m filt) a = Some x.
+Proof.
+  induction m; intuition; simpl in *;
+  destruct (eqb a a0) eqn:E.
+  - rewrite eqb_leibniz in E; subst; destruct H1; simpl in *; 
+    repeat find_injection; rewrite H2; simpl in *; rewrite eqb_refl; eauto.
+  - repeat break_match; simpl in *; 
+    try (pose proof eqb_symm; congruence);
+    simpl in *; eauto;
+    repeat (find_rewrite; intuition; eauto; try congruence).
+    rewrite eqb_symm in E; congruence.
+Qed.
+
+Global Hint Resolve filter_resolver : core.
+Global Hint Resolve filter_resolver_mapd : core.
+
+Lemma in_dec_helper : forall {A B} `{EqClass A} X l l' a (c : B),
+  map_get (minify_mapC l (fun x : A => if in_dec X x l' then true else false)) a = Some c ->
+  In a l'.
+Proof.
+  induction l; simpl in *; intuition; try congruence;
+  repeat break_if; eauto; simpl in *; 
+  repeat break_if; eauto; try rewrite eqb_leibniz in Heqb1; 
+  subst; eauto; congruence.
+Qed.
+
+Global Hint Resolve filter_resolver : core.
+
+Require Import Helpers_CvmSemantics.
+
+(* Lemma manifest_compiled_am_config_plcCb_only_unavailable : forall t st st' p, *)
+
+(* Theorem man_gen_subterm : forall (t : Term) getPl backEnv p absMan,
+  p <> getPl ->
+  map_get backEnv getPl = None ->
+  map_get (manifest_generator' p t backEnv) getPl = Some absMan ->
+  In p (knowsOf_uuid' p getPl t).
+Proof.
+  induction t; intuition; try (simpl in *; eauto; fail).
+  - unfold asp_manifest_generator, manifest_update_env, 
+      asp_manifest_update, aspid_manifest_update, update_manifest_policy_targ in *;
+    simpl in *.
+    eapply (map_set_unfolder _ getPl p); [eauto | | eapply H1 ].
+    erewrite map_get_none_iff_not_some; intros. 
+    eapply (map_set_unfolder _ getPl); eauto.
+  - admit.
+  - simpl in *. rewrite in_app_iff.
+    destruct (manifest_generator' p t1 backEnv) eqn:E1;
+    try (exfalso; eapply manifest_generator_never_empty; eauto; fail);
+    destruct (manifest_generator' p t2 (p0 :: e)) eqn:E2;
+    try (exfalso; eapply manifest_generator_never_empty; eauto; fail);
+    destruct (map_get (p0 :: e) getPl) eqn:E3.
+    * left; eapply IHt1; eauto; find_rewrite; eauto.
+    * right; eapply IHt2; eauto; find_rewrite; eauto.
+  - simpl in *. rewrite in_app_iff.
+    destruct (manifest_generator' p t1 backEnv) eqn:E1;
+    try (exfalso; eapply manifest_generator_never_empty; eauto; fail);
+    destruct (manifest_generator' p t2 (p0 :: e)) eqn:E2;
+    try (exfalso; eapply manifest_generator_never_empty; eauto; fail);
+    destruct (map_get (p0 :: e) getPl) eqn:E3.
+    * left; eapply IHt1; eauto; find_rewrite; eauto.
+    * right; eapply IHt2; eauto; find_rewrite; eauto.
+  - simpl in *. rewrite in_app_iff.
+    destruct (manifest_generator' p t1 backEnv) eqn:E1;
+    try (exfalso; eapply manifest_generator_never_empty; eauto; fail);
+    destruct (manifest_generator' p t2 (p0 :: e)) eqn:E2;
+    try (exfalso; eapply manifest_generator_never_empty; eauto; fail);
+    destruct (map_get (p0 :: e) getPl) eqn:E3.
+    * left; eapply IHt1; eauto; find_rewrite; eauto.
+    * right; eapply IHt2; eauto; find_rewrite; eauto.
+Admitted. *)
+
+Lemma callbacks_work_asps : forall absMan amLib amConf,
+  lib_supports_manifest amLib absMan ->
+  manifest_compiler absMan amLib = amConf ->
+  (forall x, In x absMan.(asps) -> 
+    forall l p t p' ev ev' res,
+      aspCb amConf (asp_paramsC x l p t) p' ev ev' = res ->
+      res = errC Runtime \/ exists r, res = resultC r
+  ).
+Proof.
+  induction absMan; simpl in *; intuition;
+  destruct res; eauto; destruct d; eauto.
+  destruct amConf; simpl in *;
+  destruct amLib; simpl in *.
+  unfold manifest_compiler in H0; repeat find_injection;
+  simpl in *.
+  repeat break_match; try congruence.
+  unfold lib_supports_manifest in *; simpl in *;
+  intuition.
+  pose proof (H0 _ H1).
+  assert ((fun x : ASP_ID =>
+             if in_dec (EqClass_impl_DecEq ASP_ID) x asps
+             then true
+             else false) x = true).
+  repeat break_match; eauto.
+  pose proof (filter_resolver _ _ ((fun x : ASP_ID =>
+             if in_dec (EqClass_impl_DecEq ASP_ID) x asps
+             then true
+             else false)) H3 H5).
+  destruct H6. 
+  assert (Some x0 = None). 
+  rewrite <- H6. rewrite <- Heqo; eauto.
+  congruence.
+Qed.
+
+Lemma add_to_list_works : forall {A} `{EqClass A} (l : list A) x,
+  In x (add_to_list l x).
+Proof.
+  induction l; simpl in *; intuition; eauto;
+  break_match; simpl in *; eauto.
+  - rewrite eqb_leibniz in *; subst; eauto.
+Qed.
+
+Local Hint Resolve add_to_list_works : core.
+
+Lemma never_change_am_conf : forall t st res st',
+  build_cvm (copland_compile t) st = (res, st') ->
+  st_AM_config st = st_AM_config st'.
+Proof.
+  induction t; simpl in *; 
+  subst; simpl in *; try rewrite eqb_refl in *;
+  repeat (
+    try break_match;
+    try monad_unfold;
+    try break_match
+    try find_injection;
+    try find_contradiction;
+    try find_injection;
+    (* repeat find_rewrite; *)
+    simpl in *; subst; intuition; 
+    eauto; try congruence);
+  repeat (
+    try (match goal with
+    | H1 : build_cvm (copland_compile ?t1) _ = _ 
+      |- _ =>
+        try (eapply IHt1 in H1)
+    | H2 : build_cvm (copland_compile ?t2) _ = _ 
+      |- _ =>
+        try (eapply IHt2 in H2)
+    end); 
+    try find_rewrite; eauto; 
+    try find_injection;
+    intuition; simpl in *; eauto
+  );
+  try (unfold remote_session, doRemote_session', do_remote in *;
+    monad_unfold; simpl in *; ff; eauto; fail);
+  try (
+    try (eapply IHt1 in Heqp; simpl in *);
+    try (eapply IHt1 in Heqp1; simpl in *);
+    try (eapply IHt1 in Heqp0; simpl in *);
+    try (eapply IHt2 in Heqp0; simpl in *);
+    try (eapply IHt2 in Heqp1; simpl in *);
+    find_rewrite; eauto).
+  - destruct a; 
+    repeat (try break_match; simpl in *; monad_unfold;
+      try find_injection; eauto).
+Qed.
+
+Definition supports_am (ac1 ac2 : AM_Config) : Prop :=
+  (forall aid l targ targid p' ev ev',
+      (forall res, 
+      ac1.(aspCb) (asp_paramsC aid l targ targid) p' ev ev' = resultC res ->
+      ac2.(aspCb) (asp_paramsC aid l targ targid) p' ev ev' = resultC res)) /\
+  (forall p, (forall res, 
+      ac1.(pubKeyCb) p = resultC res ->
+      ac2.(pubKeyCb) p = resultC res)) /\
+  (forall p, (forall res, 
+      ac1.(plcCb) p = resultC res ->
+      ac2.(plcCb) p = resultC res)) /\
+  (forall aid l targ targid p' ev ev',
+      ac1.(aspCb) (asp_paramsC aid l targ targid) p' ev ev' = errC Runtime ->
+      ac2.(aspCb) (asp_paramsC aid l targ targid) p' ev ev' = errC Runtime) /\
+  (forall p, 
+      ac1.(pubKeyCb) p = errC Runtime ->
+      ac2.(pubKeyCb) p = errC Runtime) /\
+  (forall p, 
+      ac1.(plcCb) p = errC Runtime ->
+      ac2.(plcCb) p = errC Runtime).
+
+Fixpoint am_config_support_exec (t : Term) 
+    (p : Plc) (ac : AM_Config) : Prop :=
+  match t with
+  | asp a =>
+      match a with
+      | NULL => True
+      | CPY => True
+      | SIG => 
+          forall l targ targid p' ev ev',
+          ((forall res, 
+          ac.(aspCb) (asp_paramsC sig_aspid l targ targid) p' ev ev' = resultC res) \/ 
+          ac.(aspCb) (asp_paramsC sig_aspid l targ targid) p' ev ev' = errC Runtime)
+      | HSH =>
+          forall l targ targid p' ev ev',
+          ((forall res, 
+          ac.(aspCb) (asp_paramsC hsh_aspid l targ targid) p' ev ev' = resultC res) \/ 
+          ac.(aspCb) (asp_paramsC hsh_aspid l targ targid) p' ev ev' = errC Runtime)
+      | ENC p =>
+          (forall l targ targid p' ev ev',
+          ((forall res, 
+          ac.(aspCb) (asp_paramsC enc_aspid l targ targid) p' ev ev' = resultC res) \/ 
+          ac.(aspCb) (asp_paramsC enc_aspid l targ targid) p' ev ev' = errC Runtime)) /\
+          ((forall res, ac.(pubKeyCb) p = resultC res) \/ 
+          ac.(pubKeyCb) p = errC Runtime)
+      | ASPC _ _ (asp_paramsC aspid _ _ _) =>
+          (forall l targ targid p' ev ev',
+          ((forall res, 
+          ac.(aspCb) (asp_paramsC aspid l targ targid) p' ev ev' = resultC res) \/ 
+          ac.(aspCb) (asp_paramsC aspid l targ targid) p' ev ev' = errC Runtime)) 
+      end
+  | att p' t' =>
+      ((forall res, ac.(plcCb) p' = resultC res) \/ 
+      ac.(plcCb) p' = errC Runtime)
+      (* /\ am_config_support_exec t' p' ac *)
+  | lseq t1 t2 =>
+      exists ac1 ac2,
+      (am_config_support_exec t1 p ac1) /\
+      (am_config_support_exec t2 p ac2) /\
+      supports_am ac1 ac /\
+      supports_am ac2 ac
+  | bseq _ t1 t2 =>
+      exists ac1 ac2,
+      (am_config_support_exec t1 p ac1) /\
+      (am_config_support_exec t2 p ac2) /\
+      supports_am ac1 ac /\
+      supports_am ac2 ac
+  | bpar _ t1 t2 =>
+      exists ac1 ac2,
+      (am_config_support_exec t1 p ac1) /\
+      (am_config_support_exec t2 p ac2) /\
+      supports_am ac1 ac /\
+      supports_am ac2 ac
+  end.
+
+Theorem well_formed_am_config_impl_executable : forall t p amConf,
+  am_config_support_exec t p amConf ->
+  forall st,
+  supports_am amConf (st.(st_AM_config)) ->
+  exists st', 
+    build_cvm (copland_compile t) st = (resultC tt, st') \/
+    build_cvm (copland_compile t) st = (errC (dispatch_error Runtime), st').
+Proof.
+  induction t; simpl in *; intuition; eauto.
+  - destruct a;
+    try (simpl in *; monad_unfold; eauto; fail); (* NULL, CPY *)
+    subst; simpl in *; try rewrite eqb_refl in *;
+    repeat (
+      try break_match;
+      try monad_unfold;
+      try break_match
+      try find_injection;
+      try find_contradiction;
+      try find_injection;
+      (* repeat find_rewrite; *)
+      simpl in *; subst; intuition; 
+      eauto; try congruence);
+    unfold supports_am, sig_params, enc_params, hsh_params in *; intuition;
+    try (match goal with
+    | H1 : forall _, _,
+      H2 : aspCb _ (asp_paramsC ?a ?l ?targ ?tid) ?p' ?ev ?ev' = _,
+      H3 : context[ aspCb _ _ _ _ _ = errC Runtime -> _],
+      H4 : context[ aspCb _ _ _ _ _ = resultC _ -> _]
+      |- _ =>
+        let H := fresh "H" in
+        let H' := fresh "Hx" in
+        destruct (H1 l targ tid p' ev ev') as [H | H]; 
+        [
+          (* result side *)
+          pose proof (H4 a l targ tid p' ev ev') as H';
+          erewrite H' in *; try congruence
+          |
+          (* err side *)
+          pose proof (H3 a l targ tid p' ev ev') as H';
+          intuition; find_rewrite; find_injection; eauto
+        ]
+        (* ;
+        intuition; find_rewrite; try congruence;
+        find_injection; eauto *)
+    end).
+  - subst; simpl in *; try rewrite eqb_refl in *;
+    repeat (
+      unfold remote_session, doRemote_session', do_remote in *;
+      try break_match;
+      try monad_unfold;
+      try break_match
+      try find_injection;
+      try find_contradiction;
+      try find_injection;
+      (* repeat find_rewrite; *)
+      simpl in *; subst; intuition; 
+      eauto; try congruence);
+    unfold supports_am in *; intuition;
+    erewrite H2 in *; try congruence.
+  - subst; simpl in *; try rewrite eqb_refl in *;
+    repeat (
+      unfold remote_session, doRemote_session', do_remote in *;
+      try break_match;
+      try monad_unfold;
+      try break_match
+      try find_injection;
+      try find_contradiction;
+      try find_injection;
+      (* repeat find_rewrite; *)
+      simpl in *; subst; intuition; 
+      eauto; try congruence);
+    unfold supports_am in *; intuition;
+    erewrite H6 in *; try congruence;
+    find_injection; eauto.
+  - subst; simpl in *; try rewrite eqb_refl in *;
+    repeat (
+      try break_match;
+      try monad_unfold;
+      try break_match
+      try find_injection;
+      try find_contradiction;
+      try find_injection;
+      (* repeat find_rewrite; *)
+      simpl in *; subst; intuition; 
+      eauto; try congruence).
+    * destruct H as [ac1 [ac2 H]]; intuition.
+      pose proof (IHt1 _ _ H0).
+      destruct (IHt1 _ _ H0).
+      destruct (IHt2 _ _ H st eq_refl); 
+      intuition; eauto;
+      repeat find_rewrite;
+      repeat find_injection; eauto.
+    * destruct (IHt1 _ _ H0 st eq_refl);
+      destruct H; find_rewrite; find_injection; eauto;
+      assert (st_AM_config x = st_AM_config st) by
+          (symmetry;
+          eapply never_change_am_conf; eauto);
+          destruct (IHt2 _ _ H1 x H); intuition; eauto;
+         find_rewrite; find_injection; eauto.
+  - subst; simpl in *; try rewrite eqb_refl in *;
+    repeat (
+      try break_match;
+      try monad_unfold;
+      try break_match
+      try find_injection;
+      try find_contradiction;
+      try find_injection;
+      (* repeat find_rewrite; *)
+      simpl in *; subst; intuition; 
+      eauto; try congruence);
+      match goal with
+      | H1 : am_config_support_exec t1 _ ?amConf,
+        H2 : build_cvm (copland_compile t1) ?st = _
+        |- _ =>
+          pose proof (eq_sym (never_change_am_conf _ _ _ _ H2));
+          simpl in *;
+          pose proof (IHt1 _ _ H1 st); 
+          repeat (
+            try break_exists;
+            intuition);
+          try find_rewrite;
+          try find_injection; eauto; try congruence
+      end;
+      match goal with
+      | H1 : am_config_support_exec t2 _ ?amConf,
+        H2 : build_cvm (copland_compile t2) ?st = _
+        |- _ =>
+          pose proof (eq_sym (never_change_am_conf _ _ _ _ H2));
+          simpl in *;
+          pose proof (IHt2 _ _ H1 st); 
+          repeat (
+            try break_exists;
+            intuition);
+          try find_rewrite;
+          try find_injection; eauto; try congruence
+      end; simpl in *.
+  - subst; simpl in *; try rewrite eqb_refl in *;
+    repeat (
+      try break_match;
+      try monad_unfold;
+      try break_match
+      try find_injection;
+      try find_contradiction;
+      try find_injection;
+      (* repeat find_rewrite; *)
+      simpl in *; subst; intuition; 
+      eauto; try congruence);
+      match goal with
+      | H1 : am_config_support_exec t1 _ ?amConf,
+        H2 : build_cvm (copland_compile t1) ?st = _
+        |- _ =>
+          pose proof (eq_sym (never_change_am_conf _ _ _ _ H2));
+          simpl in *;
+          pose proof (IHt1 _ _ H1 st); 
+          repeat (
+            try break_exists;
+            intuition);
+          try find_rewrite;
+          try find_injection; eauto; try congruence
+      end;
+      match goal with
+      | H1 : am_config_support_exec t2 _ ?amConf,
+        H2 : build_cvm (copland_compile t2) ?st = _
+        |- _ =>
+          pose proof (eq_sym (never_change_am_conf _ _ _ _ H2));
+          simpl in *;
+          pose proof (IHt2 _ _ H1 st); 
+          repeat (
+            try break_exists;
+            intuition);
+          try find_rewrite;
+          try find_injection; eauto; try congruence
+      end; simpl in *.
+Qed.
+
+Lemma in_add_to_list : forall {A} `{EqClass A} (l : list A) x x',
+  In x l ->
+  In x (add_to_list l x').
+Proof.
+  induction l; simpl in *; intuition; eauto;
+  subst; eauto.
+  - break_match; simpl in *; eauto.
+  - break_match; simpl in *; eauto.
+Qed.
+
+Local Hint Resolve in_add_to_list : core.
+
+(* Theorem gen_man_preserves : forall (t : Term) (p : Plc) 
+  (my_abstract_plc : Plc) asps uuidPlcs' pubKeyPlcs targetPlcs policy,
+  (* In p (uuidPlcs (st)) -> *)
+  In p (uuidPlcs
+     (generate_manifest' t p
+        {|
+          my_abstract_plc := my_abstract_plc;
+          asps := asps;
+          uuidPlcs := add_to_list (uuidPlcs') p;
+          pubKeyPlcs := pubKeyPlcs;
+          targetPlcs := targetPlcs ;
+          policy := policy 
+        |})) .
+        (* <->
+  In p (add_to_list (uuidPlcs
+     (generate_manifest' t p
+        {|
+          my_abstract_plc := my_abstract_plc ;
+          asps := asps ;
+          uuidPlcs := uuidPlcs' ;
+          pubKeyPlcs := pubKeyPlcs ;
+          targetPlcs := targetPlcs ;
+          policy := policy 
+        |})) p). *)
+Proof.
+  induction t.
+  (* induction t; simpl in *; intuition; eauto.
+  - destruct a; ff.
+  - destruct (in_dec (EqClass_impl_DecEq _) p0 (uuidPlcs
+            (generate_manifest' t p
+               {|
+                 my_abstract_plc := my_abstract_plc;
+                 asps := asps;
+                 uuidPlcs := add_to_list uuidPlcs' p;
+                 pubKeyPlcs := pubKeyPlcs;
+                 targetPlcs := targetPlcs;
+                 policy := policy
+               |}))).
+    *  *)
+Admitted. *)
+
+(* Local Hint Resolve gen_man_preserves : core. *)
+
+Theorem generate_manifest'_preserves_plc : forall t p st st',
+  generate_manifest' t p st = st' ->
+  st.(my_abstract_plc) = st'.(my_abstract_plc).
+Proof.
+  induction t; simpl in *; intuition; eauto;
+  repeat break_match; subst; eauto;
+  try (destruct (generate_manifest' t1 p st) eqn:E1;
+    eapply IHt1 in E1; simpl in *;
+    destruct (generate_manifest' t2 p {|
+       my_abstract_plc := my_abstract_plc;
+       asps := asps;
+       uuidPlcs := uuidPlcs;
+       pubKeyPlcs := pubKeyPlcs;
+       targetPlcs := targetPlcs;
+       policy := policy
+     |}) eqn:E2;
+    eapply IHt2 in E2; simpl in *; subst; eauto).
+Qed.
+
+Theorem generate_manifest'_preserves_asps : forall t p st x st',
+  p = my_abstract_plc st ->
+  In x (asps st) ->
+  generate_manifest' t p st = st' ->
+  In x (asps st').
+Proof.
+  induction t; simpl in *; intuition; eauto;
+  subst; try rewrite eqb_refl in *; simpl in *;
+    repeat break_match; simpl in *;
+    try find_injection; eauto.
+  - destruct (generate_manifest' t1 (my_abstract_plc st) st) eqn:E1;
+    simpl in *.
+    eapply IHt1 in E1 as H'; eauto.
+    destruct (generate_manifest' t2 (Manifest.my_abstract_plc st) {|
+          my_abstract_plc := my_abstract_plc;
+          asps := asps;
+          uuidPlcs := uuidPlcs;
+          pubKeyPlcs := pubKeyPlcs;
+          targetPlcs := targetPlcs;
+          policy := policy
+        |}) eqn:E2; simpl in *; eauto.
+    eapply IHt2 in E2; eauto.
+    simpl in *.
+    eapply generate_manifest'_preserves_plc in E1;
+    eapply generate_manifest'_preserves_plc in E2;
+    simpl in *; subst; eauto.
+  - destruct (generate_manifest' t1 (my_abstract_plc st) st) eqn:E1;
+    simpl in *.
+    eapply IHt1 in E1 as H'; eauto.
+    destruct (generate_manifest' t2 (Manifest.my_abstract_plc st) {|
+          my_abstract_plc := my_abstract_plc;
+          asps := asps;
+          uuidPlcs := uuidPlcs;
+          pubKeyPlcs := pubKeyPlcs;
+          targetPlcs := targetPlcs;
+          policy := policy
+        |}) eqn:E2; simpl in *; eauto.
+    eapply IHt2 in E2; eauto.
+    simpl in *.
+    eapply generate_manifest'_preserves_plc in E1;
+    eapply generate_manifest'_preserves_plc in E2;
+    simpl in *; subst; eauto.
+  - destruct (generate_manifest' t1 (my_abstract_plc st) st) eqn:E1;
+    simpl in *.
+    eapply IHt1 in E1 as H'; eauto.
+    destruct (generate_manifest' t2 (Manifest.my_abstract_plc st) {|
+          my_abstract_plc := my_abstract_plc;
+          asps := asps;
+          uuidPlcs := uuidPlcs;
+          pubKeyPlcs := pubKeyPlcs;
+          targetPlcs := targetPlcs;
+          policy := policy
+        |}) eqn:E2; simpl in *; eauto.
+    eapply IHt2 in E2; eauto.
+    simpl in *.
+    eapply generate_manifest'_preserves_plc in E1;
+    eapply generate_manifest'_preserves_plc in E2;
+    simpl in *; subst; eauto.
+Qed.
+
+Theorem lib_supports_cumul : 
+  forall t p st,
+  forall amLib absMan,
+  lib_supports_manifest amLib absMan ->
+  generate_manifest' t p st = absMan ->
+  lib_supports_manifest amLib st.
+Proof.
+  induction t; simpl in *; intuition; eauto;
+  try (repeat break_match; subst; eauto;
+  unfold lib_supports_manifest in *; intuition;
+  simpl in *; eauto; fail).
+Qed.
+
+Theorem man_gen_comp_works : forall t p backMan absMan amLib,
+  lib_supports_manifest amLib backMan ->
+  p = backMan.(my_abstract_plc) ->
+  generate_manifest' t p backMan = absMan ->
+  (* forall amLib, *)
+  lib_supports_manifest amLib absMan ->
+  (forall amConf,
+    manifest_compiler absMan amLib = amConf ->
+    am_config_support_exec t p amConf
+  ).
+Proof.
+  induction t; simpl in *; intros.
+  - rewrite H0 in *;
+    rewrite eqb_refl in *;
+    unfold lib_supports_manifest, manifest_compiler in *;
+    destruct amConf; find_injection; simpl in *;
+    repeat (
+      try unfold generate_PubKey_dispatcher in *;
+      repeat break_match; repeat find_injection;
+      simpl in *; intuition; eauto; try congruence
+    );
+    try (match goal with
+    | H:  context[ map_get (minify_mapC ?l ?filt) ?a],
+      H1: forall a' : Plc, _ -> (exists x : _, map_get _ _ = Some x) |- _ => 
+      assert (CO : exists x, map_get (minify_mapC l filt) a = Some x)
+      ;
+        [
+        eapply filter_resolver; eauto;
+        repeat break_match; intuition; try congruence
+        | 
+        rewrite H in CO; destruct CO; congruence
+      ]
+    | H:  context[ map_get (minify_mapD ?l ?filt) ?a],
+      H1: forall a' : Plc, _ -> (exists x : _, map_get _ _ = Some x) |- _ => 
+      assert (CO : exists x, map_get (minify_mapD l filt) a = Some x)
+      ;
+        [
+        eapply filter_resolver_mapd; eauto;
+        repeat break_match; intuition; try congruence
+        | 
+        rewrite H in CO; destruct CO; congruence
+      ]
+    end).
+  - unfold lib_supports_manifest, manifest_compiler in *;
+    destruct amConf; find_injection; simpl in *;
+    repeat (
+      try unfold generate_Plc_dispatcher in *;
+      repeat break_match; repeat find_injection;
+      simpl in *; intuition; eauto; try congruence
+    );
+    try (match goal with
+    | H:  context[ map_get (minify_mapC ?l ?filt) ?a],
+      H1: forall a' : Plc, _ -> (exists x : _, map_get _ _ = Some x) |- _ => 
+      assert (CO : exists x, map_get (minify_mapC l filt) a = Some x)
+      ;
+        [
+        eapply filter_resolver; eauto;
+        repeat break_match; intuition; try congruence
+        | 
+        rewrite H in CO; destruct CO; congruence
+      ]
+    | H:  context[ map_get (minify_mapD ?l ?filt) ?a],
+      H1: forall a' : Plc, _ -> (exists x : _, map_get _ _ = Some x) |- _ => 
+      assert (CO : exists x, map_get (minify_mapD l filt) a = Some x)
+      ;
+        [
+        eapply filter_resolver_mapd; eauto;
+        repeat break_match; intuition; try congruence
+        | 
+        rewrite H in CO; destruct CO; congruence
+      ]
+    end).
+  - destruct (generate_manifest' t1 p backMan) eqn:E1.
+    assert (lib_supports_manifest amLib
+      {|
+        my_abstract_plc := my_abstract_plc;
+        asps := asps;
+        uuidPlcs := uuidPlcs;
+        pubKeyPlcs := pubKeyPlcs;
+        targetPlcs := targetPlcs;
+        policy := policy
+      |}). {
+        eapply lib_supports_cumul; eauto.
+    }
+    pose proof (IHt1 _ _ _ _ H H0 E1 H4).
+    
+    eapply lib_supports_cumul with (amLib := amLib) in E1 as HL1.
+    pose proof (IHt1 _ _ _ H E1 amLib).
+    eapply 
+
+    (* pose proof (IHt1 _ _ _ H E1 amLib). *)
+    assert (lib_supports_manifest amLib
+       {|
+         my_abstract_plc := my_abstract_plc;
+         asps := asps;
+         uuidPlcs := uuidPlcs;
+         pubKeyPlcs := pubKeyPlcs;
+         targetPlcs := targetPlcs;
+         policy := policy
+       |}). {
+       unfold lib_supports_manifest in *; simpl in *;
+       intuition; eauto.
+       - 
+        eapply H3.
+         pose proof (generate_manifest'_preserves_asps 
+          t1 p backMan a ({|
+            my_abstract_plc := my_abstract_plc;
+            asps := asps;
+            uuidPlcs := uuidPlcs;
+            pubKeyPlcs := pubKeyPlcs;
+            targetPlcs := targetPlcs;
+            policy := policy
+          |})
+         ). intuition.
+          
+    }
+
+
+    pose proof (IHt2 _ _ _ H H0).
+    repeat break_match; repeat find_injection;
+    simpl in *; intuition; eauto; try congruence.
+    * rewrite <- H0 in *; simpl in *;
+      unfold lib_supports_manifest, manifest_compiler in *.
+      destruct amConf; find_injection; simpl in *.
+
+
+  induction t; simpl in *; intuition; subst; eauto;
+  repeat rewrite eqb_refl in *.
+  - unfold generate_PubKey_dispatcher;
+    destruct a; intuition; simpl in *;
+    try (try (destruct a); 
+    simpl in *; intuition;
+    repeat break_match; simpl in *; eauto;
+    unfold lib_supports_manifest in *; simpl in *; intuition;
+    (* pose proof (filter_resolver (Local_ASPS amLib)). *)
+    try (match goal with
+    | H:  context[ map_get (minify_mapC ?l ?filt) ?a],
+      H1: forall a' : Plc, _ -> (exists x : _, map_get _ _ = Some x) |- _ => 
+      assert (CO : exists x, map_get (minify_mapC l filt) a = Some x)
+      ;
+        [
+        eapply filter_resolver; eauto;
+        repeat break_match; intuition; try congruence
+        | 
+        rewrite H in CO; destruct CO; congruence
+      ]
+    end); fail).
+    * unfold generate_PubKey_dispatcher, lib_supports_manifest in *; 
+      simpl in *; intuition;
+      repeat break_match; simpl in *; eauto;
+      match goal with
+      | H:  context[ map_get (minify_mapD ?l ?filt) ?a],
+        H1: forall a' : Plc, _ -> (exists x : _, map_get _ _ = Some x) |- _ => 
+        assert (CO : exists x, map_get (minify_mapD l filt) a = Some x)
+        ;
+          [
+          eapply filter_resolver_mapd; eauto;
+          repeat break_match; intuition; try congruence
+          | 
+          rewrite H in CO; destruct CO; congruence
+        ]
+      end.
+  - repeat (
+      unfold lib_supports_manifest, generate_Plc_dispatcher in *; simpl in *; intuition; eauto; try congruence).
+    repeat break_match; simpl in *; eauto.
+    match goal with
+    | H:  context[ map_get (minify_mapD ?l ?filt) ?a],
+      H1: forall a' : Plc, _ -> (exists x : _, map_get _ _ = Some x) |- _ => 
+      assert (CO : exists x, map_get (minify_mapD l filt) a = Some x)
+      ;
+        [
+        eapply filter_resolver_mapd; eauto;
+        repeat break_match; intuition; try congruence
+        | 
+        rewrite H in CO; destruct CO; congruence
+      ]
+    end; eauto;
+    pose proof (H1 _ (gen_man_preserves _ _ _ _ _ _ _ _));
+    try (exfalso; eauto; fail); eauto.
+    
+  - pose proof (IHt (my_abstract_plc backMan) backMan).
+    repeat (
+      unfold lib_supports_manifest, generate_Plc_dispatcher in *; simpl in *; intuition; eauto; try congruence);
+    repeat break_match; simpl in *; eauto.
+    clear IHt.
+    unfold am_config_support_exec; simpl in *.
+    destruct ((generate_manifest' t p
+          {|
+            my_abstract_plc := my_abstract_plc backMan;
+            asps := asps backMan;
+            uuidPlcs := add_to_list (uuidPlcs backMan) p;
+            pubKeyPlcs := pubKeyPlcs backMan;
+            targetPlcs := targetPlcs backMan;
+            policy := policy backMan
+          |})) eqn:E; eauto.
+    assert (p = Manifest.my_abstract_plc backMan). admit.
+    destruct ((manifest_compiler
+     {|
+       my_abstract_plc := my_abstract_plc;
+       asps := asps;
+       uuidPlcs := uuidPlcs;
+       pubKeyPlcs := pubKeyPlcs;
+       targetPlcs := targetPlcs;
+       policy := policy
+     |} amLib)) eqn:E1.
+    pose proof (IHt p {|
+        my_abstract_plc := Manifest.my_abstract_plc backMan;
+        asps := Manifest.asps backMan;
+        uuidPlcs := add_to_list (Manifest.uuidPlcs backMan) p;
+        pubKeyPlcs := Manifest.pubKeyPlcs backMan;
+        targetPlcs := Manifest.targetPlcs backMan;
+        policy := Manifest.policy backMan
+      |} _ H E _ H1 _ E1). eauto.
+    repeat (
+      unfold lib_supports_manifest, generate_Plc_dispatcher in *; simpl in *; intuition; eauto; try congruence).
+    repeat break_match; simpl in *; eauto.
+    match goal with
+    | H:  context[ map_get (minify_mapD ?l ?filt) ?a],
+      H1: forall a' : Plc, _ -> (exists x : _, map_get _ _ = Some x) |- _ => 
+      assert (CO : exists x, map_get (minify_mapD l filt) a = Some x)
+      ;
+        [
+        eapply filter_resolver_mapd; eauto;
+        repeat break_match; intuition; try congruence
+        | 
+        rewrite H in CO; destruct CO; congruence
+      ]
+    end; eauto;
+    pose proof (H1 _ (gen_man_preserves _ _ _ _ _ _ _ _));
+    try (exfalso; eauto; fail); eauto.
+
+    
+    
+
+      eapply H1; eauto.
+    try (destruct a); 
+    simpl in *; intuition;
+    repeat break_match; simpl in *; eauto;
+    unfold lib_supports_manifest in *; simpl in *; intuition;
+    (* pose proof (filter_resolver (Local_ASPS amLib)). *)
+    match goal with
+    | H:  context[ map_get (minify_mapC ?l ?filt) ?a],
+      H1: forall a' : Plc, _ -> (exists x : _, map_get _ _ = Some x) |- _ => 
+      assert (CO : exists x, map_get (minify_mapC l filt) a = Some x)
+      ;
+        [
+        eapply filter_resolver; eauto;
+        repeat break_match; intuition; try congruence
+        | 
+        rewrite H in CO; destruct CO; congruence
+      ]
+    end.
+    * simpl in *; intuition;
+      repeat break_match; simpl in *; eauto;
+      unfold lib_supports_manifest in *; simpl in *; intuition;
+      (* pose proof (filter_resolver (Local_ASPS amLib)). *)
+      match goal with
+      | H:  context[ map_get (minify_mapC ?l ?filt) ?a],
+        H1: forall a' : Plc, _ -> (exists x : _, map_get _ _ = Some x) |- _ => 
+        assert (CO : exists x, map_get (minify_mapC l filt) a = Some x)
+        ;
+         [
+          eapply filter_resolver; eauto;
+          repeat break_match; intuition; try congruence
+          | 
+          rewrite H in CO; destruct CO; congruence
+        ]
+      end.
+      eapply filter_resolver.  eapply H; eauto.
+
+
+   manifest_generator' p t backEnv = envM ->
+  (forall p' absMan, 
+    map_get backEnv p' = None ->
+    map_get envM p' = Some absMan ->
+    (forall amLib amConf, 
+      lib_supports_manifest amLib absMan ->
+      manifest_compiler absMan amLib = amConf ->
+      
+    )
+  ).
+.
+Proof.
+  
+Qed.
